incr/FAA_A.v
@@ -1,0 +1,40 @@
+Require Import CRIS.
+Require Import ImpPrelude IncrHeader MemHeader MemA SchA SchTactics SchHeader.
+
+Module FaaA. Section FaaA.
+  Context `{!invG α Σ Γ, !subG Γ Σ, !sinvG Σ Γ α β τ, !memGΓ Γ}.
+  Context `{!SchAGΣ Σ, !SchAGΓ Γ}.
+
+  Definition faa2_spec u : fspec :=
+    w_fspec_sch u (fspec_simple (λ '(b, ofs), (λ arg, ⌜arg = [Vptr b ofs]↑⌝, λ ret, ⌜ret = tt↑⌝)))%I.
+
+  Definition spc u : alist string fspec :=
+    [(FaaHdr.faa2, faa2_spec u)].
+
+  Definition scopes : list string := [].
+
+  Definition faa2 : list val → itree hmodE unit :=
+    λ arg,
+      '(b, ofs) : mblock * ptrofs <- (pargs [Tptr] arg)?;;
+      𝒴;;;
+        'v : Z <- trigger (Take Z);;
+        trigger (Assume ((b, ofs) ↦ Vint v));;;
+        trigger (Guarantee ((b, ofs) ↦ Vint (v + 1)));;;
+      𝒴;;;
+        'v : Z <- trigger (Take Z);;
+        trigger (Assume ((b, ofs) ↦ Vint v));;;
+        trigger (Guarantee ((b, ofs) ↦ Vint (v + 1)));;;
+      𝒴;;; Ret tt.
+
+  Definition fnsems u := [(FaaHdr.faa2, (scopes, mk_specbody (faa2_spec u) (cfunN faa2)))].
+
+  Program Definition Mod u : SMod.t := {|
+    SMod.scopes := scopes;
+    SMod.fnsems := fnsems u;
+    SMod.initial_st := [];
+  |}.
+  Solve All Obligations with prove_scope.
+  Next Obligation. prove_nodup. Qed.
+
+  Definition t u spc : HMod.t := Seal.sealing CRIS (SMod.to_hmod (wsim_ginv u ⊤) spc (Mod u)).
+End FaaA. End FaaA.
