incr/FAA_I.v
@@ -1,0 +1,26 @@
+Require Import CRIS.
+Require Import ImpPrelude IncrHeader MemHeader MemA SchA SchTactics SchHeader.
+
+Module FaaI. Section FaaI.
+  Context {Σ : GRA}.
+
+  Definition scopes : list string := [].
+
+  Definition faa2 : list val → itree pmodE unit :=
+    λ arg,
+      𝒴;;; '_ : val <- MemHdr.faa arg;;
+      𝒴;;; '_ : val <- MemHdr.faa arg;;
+      𝒴;;; Ret tt.
+
+  Definition fnsems := [(FaaHdr.faa2, (scopes, cfunU faa2))].
+
+  Program Definition Mod : PMod.t := {|
+    PMod.scopes := scopes;
+    PMod.fnsems := fnsems;
+    PMod.initial_st := [];
+  |}.
+  Solve All Obligations with prove_scope.
+  Next Obligation. prove_nodup. Qed.
+
+  Definition t : HMod.t := Seal.sealing CRIS (PMod.to_hmod Mod).
+End FaaI. End FaaI.
