incr/FAA_IAproof.v
@@ -1,67 +1,6 @@
 Require Import CRIS.
 Require Import ImpPrelude IncrHeader MemHeader MemA SchA SchTactics SchHeader.
-
-Module FaaI. Section FaaI.
-  Context {Σ : GRA}.
-
-  Definition scopes : list string := [].
-
-  Definition faa : list val → itree pmodE unit :=
-    λ arg,
-      𝒴;;; '_ : val <- MemHdr.faa arg;;
-      𝒴;;; '_ : val <- MemHdr.faa arg;;
-      𝒴;;; Ret tt.
-
-  Definition fnsems := [(FaaHdr.faa, (scopes, cfunU faa))].
-
-  Program Definition Mod : PMod.t := {|
-    PMod.scopes := scopes;
-    PMod.fnsems := fnsems;
-    PMod.initial_st := [];
-  |}.
-  Solve All Obligations with prove_scope.
-  Next Obligation. prove_nodup. Qed.
-
-  Definition t : HMod.t := Seal.sealing CRIS (PMod.to_hmod Mod).
-End FaaI. End FaaI.
-
-Module FaaA. Section FaaA.
-  Context `{!invG α Σ Γ, !subG Γ Σ, !sinvG Σ Γ α β τ, !memGΓ Γ}.
-  Context `{!SchAGΣ Σ, !SchAGΓ Γ}.
-
-  Definition faa_spec u : fspec :=
-    w_fspec_sch u (fspec_simple (λ '(b, ofs), (λ arg, ⌜arg = [Vptr b ofs]↑⌝, λ ret, ⌜ret = tt↑⌝)))%I.
-
-  Definition spc u : alist string fspec :=
-    [(FaaHdr.faa, faa_spec u)].
-
-  Definition scopes : list string := [].
-
-  Definition faa : list val → itree hmodE unit :=
-    λ arg,
-      '(b, ofs) : mblock * ptrofs <- (pargs [Tptr] arg)?;;
-      𝒴;;;
-        'v : Z <- trigger (Take Z);;
-        trigger (Assume ((b, ofs) ↦ Vint v));;;
-        trigger (Guarantee ((b, ofs) ↦ Vint (v + 1)));;;
-      𝒴;;;
-        'v : Z <- trigger (Take Z);;
-        trigger (Assume ((b, ofs) ↦ Vint v));;;
-        trigger (Guarantee ((b, ofs) ↦ Vint (v + 1)));;;
-      𝒴;;; Ret tt.
-
-  Definition fnsems u := [(FaaHdr.faa, (scopes, mk_specbody (faa_spec u) (cfunN faa)))].
-
-  Program Definition Mod u : SMod.t := {|
-    SMod.scopes := scopes;
-    SMod.fnsems := fnsems u;
-    SMod.initial_st := [];
-  |}.
-  Solve All Obligations with prove_scope.
-  Next Obligation. prove_nodup. Qed.
-
-  Definition t u spc : HMod.t := Seal.sealing CRIS (SMod.to_hmod (wsim_ginv u ⊤) spc (Mod u)).
-End FaaA. End FaaA.
+Require Import FAA_I FAA_A.
 
 Module FaaIA. Section FaaIA.
   Context `{!invG α Σ Γ, !subG Γ Σ, !sinvG Σ Γ α β τ}.
@@ -79,7 +18,7 @@ Module FaaIA. Section FaaIA.
   Local Definition MA := (FaaA ★ MemA).
   Local Definition MI := (FaaI ★ MemA).
 
-  Lemma faa_simF : HSim.sim_fun open MA MI IstFull FaaHdr.faa.
+  Lemma faa2_simF : HSim.sim_fun open MA MI IstFull FaaHdr.faa2.
   Proof.
     init_simF u_s 0.
     steps_l. iDestruct "ASM" as "[TID [-> ->]]". hss. rename q3 into b, q4 into ofs, q1 into tid.
@@ -136,6 +75,6 @@ Module FaaIA. Section FaaIA.
   Proof.
     init_sim.
     { iIntros "_"; iExists [], [], [], []; eauto. }
-    { eapply faa_simF. }
+    { eapply faa2_simF. }
   Qed.
 End FaaIA. End FaaIA.
